coq/extract.v
@@ -23,7 +23,7 @@ Extract Inlined Constant projT1 => "fst".
 Extract Inlined Constant projT2 => "snd".
 
 Extraction Inline eq_dec dc_dec.
-Extraction Inline dec.OneDec dec.isEq2_obligation_1 dec.PairDec_obligation_1.
+Extraction Inline dec.OneDec dec.isEq2_obligation_1 dec.DepPairDec_obligation_1.
 Extraction Inline finite.asDec_obligation_1 finite.asDec abstraction.newPredDec_obligation_1.
 
 Extraction "/tmp/extract.ml" transfo.mlTransform.
